fstar/treesync/symbolic/MLS.TreeSync.Symbolic.API.GroupManager.fst
@@ -6,6 +6,8 @@ open DY.Lib
 open MLS.NetworkTypes
 open MLS.Symbolic
 
+#set-options "--fuel 0 --ifuel 0"
+
 (*** Group manager types & invariants ***)
 
 [@@ with_bytes dy_bytes]
@@ -31,6 +33,7 @@ instance group_manager_types: map_types group_manager_key group_manager_value = 
   ps_value_t = ps_group_manager_value;
 }
 
+#push-options "--ifuel 1"
 val group_manager_pred: {|crypto_invariants|} -> map_predicate group_manager_key group_manager_value #_
 let group_manager_pred #ci = {
   pred = (fun tr prin state_id key value ->
@@ -39,6 +42,7 @@ let group_manager_pred #ci = {
   pred_later = (fun tr1 tr2 prin state_id key value -> ());
   pred_knowable = (fun tr prin state_id key value -> ());
 }
+#pop-options
 
 val has_group_manager_invariant: {|protocol_invariants|} -> prop
 let has_group_manager_invariant #invs =
